faster verifier simulation proof

verifier/simulation/correct_bpf_verifier_opcode_alu32_imm.v
@@ -20,40 +20,80 @@ bpf_verifier_opcode_alu32_imm
 *)
 Open Scope Z_scope.
 
-Lemma bpf_verifier_opcode_alu32_imm_match:
-  forall c
-    (Halu : match c with
-       | 4%nat => ADD32_IMM
-       | 20%nat => SUB32_IMM
-       | 36%nat => MUL32_IMM
-       | 52%nat => DIV32_IMM
-       | 68%nat => OR32_IMM
-       | 84%nat => AND32_IMM
-       | 100%nat => LSH32_IMM
-       | 116%nat => RSH32_IMM
-       | 132%nat => NEG32_IMM
-       | 148%nat => MOD32_IMM
-       | 164%nat => XOR32_IMM
-       | 180%nat => MOV32_IMM
-       | 196%nat => ARSH32_IMM
-       | _ => ALU32_IMM_ILLEGAL
-       end = ALU32_IMM_ILLEGAL),
-          4   <> (Z.of_nat c) /\
-          20  <> (Z.of_nat c) /\
-          36  <> (Z.of_nat c) /\
-          52  <> (Z.of_nat c) /\
-          68  <> (Z.of_nat c) /\
-          84  <> (Z.of_nat c) /\
-          100 <> (Z.of_nat c) /\
-          116 <> (Z.of_nat c) /\
-          132 <> (Z.of_nat c) /\
-          148 <> (Z.of_nat c) /\
-          164 <> (Z.of_nat c) /\
-          180 <> (Z.of_nat c) /\
-          196 <> (Z.of_nat c).
+Definition opcode_alu32_imm_if (op: nat) : opcode_alu32_imm :=
+  if Nat.eqb op 4%nat then ADD32_IMM
+  else if Nat.eqb op 20%nat then SUB32_IMM
+  else if Nat.eqb op 36%nat then MUL32_IMM
+  else if Nat.eqb op 52%nat then DIV32_IMM
+  else if Nat.eqb op 68%nat then OR32_IMM
+  else if Nat.eqb op 84%nat then AND32_IMM
+  else if Nat.eqb op 100%nat then LSH32_IMM
+  else if Nat.eqb op 116%nat then RSH32_IMM
+  else if Nat.eqb op 132%nat then NEG32_IMM
+  else if Nat.eqb op 148%nat then MOD32_IMM
+  else if Nat.eqb op 164%nat then XOR32_IMM
+  else if Nat.eqb op 180%nat then MOV32_IMM
+  else if Nat.eqb op 196%nat then ARSH32_IMM
+  else ALU32_IMM_ILLEGAL.
+
+Lemma opcode_alu32_imm_eqb_eq : forall a b,
+    opcode_alu32_imm_eqb a b = true -> a = b.
+Proof.
+  destruct a,b ; simpl ;congruence.
+Qed.
+
+Lemma lift_opcode_alu32_imm :
+  forall (E: nat -> opcode_alu32_imm)
+         (F: nat -> opcode_alu32_imm) n,
+    ((fun n => opcode_alu32_imm_eqb (E n) (F n) = true) n) <->
+      (((fun n => opcode_alu32_imm_eqb (E n) (F n)) n) = true).
 Proof.
   intros.
-  do 197 (destruct c; [inversion Halu; split_conj | ]).
+  simpl. reflexivity.
+Qed.
+
+Lemma byte_to_opcode_alu32_imm_if_same:
+  forall (op: nat),
+    (op <= 255)%nat ->
+    nat_to_opcode_alu32_imm op = opcode_alu32_imm_if op.
+Proof.
+  intros.
+  unfold nat_to_opcode_alu32_imm, opcode_alu32_imm_if.
+  apply opcode_alu32_imm_eqb_eq.
+  match goal with
+  | |- ?A = true => set (P := A)
+  end.
+  pattern op in P.
+  match goal with
+  | P := ?F op |- _=>
+      apply (Forall_exec_spec F 255)
+  end.
+  vm_compute.
+  reflexivity.
+  assumption.
+Qed.
+
+Lemma bpf_verifier_opcode_alu32_imm_match:
+  forall op
+    (Hop: (op <= 255)%nat)
+    (Halu : nat_to_opcode_alu32_imm op = ALU32_IMM_ILLEGAL),
+        4   <> (Z.of_nat op) /\
+        20  <> (Z.of_nat op) /\
+        36  <> (Z.of_nat op) /\
+        52  <> (Z.of_nat op) /\
+        68  <> (Z.of_nat op) /\
+        84  <> (Z.of_nat op) /\
+        100 <> (Z.of_nat op) /\
+        116 <> (Z.of_nat op) /\
+        132 <> (Z.of_nat op) /\
+        148 <> (Z.of_nat op) /\
+        164 <> (Z.of_nat op) /\
+        180 <> (Z.of_nat op) /\
+        196 <> (Z.of_nat op).
+Proof.
+  intros.
+  rewrite byte_to_opcode_alu32_imm_if_same in Halu; auto.
+  unfold opcode_alu32_imm_if in Halu.
   change 4   with (Z.of_nat 4%nat).
   change 20  with (Z.of_nat 20%nat).
   change 36  with (Z.of_nat 36%nat).
@@ -67,8 +107,26 @@ Proof.
   change 164 with (Z.of_nat 164%nat).
   change 180 with (Z.of_nat 180%nat).
   change 196 with (Z.of_nat 196%nat).
-  repeat (split; [intro Hfalse; apply Nat2Z.inj in Hfalse; inversion Hfalse |]).
-  intro Hfalse; apply Nat2Z.inj in Hfalse; inversion Hfalse.
+Ltac simpl_neq :=
+  let Hfalse := fresh "Hfalse" in
+  match goal with
+  | H : (if ?X then _ else _) = _ |- _ /\ _ =>
+    split; [destruct X eqn: Hnew; [inversion H |
+      rewrite Nat.eqb_neq in Hnew;
+      intro Hfalse; apply Hnew;
+      symmetry in Hfalse;
+      apply Nat2Z.inj in Hfalse;
+      assumption]
+    | destruct X eqn: Hnew; [inversion H| clear Hnew]]
+  | H : (if ?X then _ else _) = _ |- _ =>
+    destruct X eqn: Hnew; [inversion H |
+      rewrite Nat.eqb_neq in Hnew;
+      intro Hfalse; apply Hnew;
+      symmetry in Hfalse;
+      apply Nat2Z.inj in Hfalse;
+      assumption]
+  end.
+  repeat simpl_neq.
 Qed.
 
 
@@ -809,8 +867,7 @@ Ltac correct_forward L :=
 
         unfold select_switch.
         unfold select_switch_case.
-        unfold nat_to_opcode_alu32_imm in Halu.
-        apply bpf_verifier_opcode_alu32_imm_match in Halu.
+        apply bpf_verifier_opcode_alu32_imm_match in Halu; auto.
         destruct Halu as (Hfirst & Halu). eapply Coqlib.zeq_false in Hfirst. rewrite Hfirst; clear Hfirst.
         repeat match goal with
         | H: ?X <> ?Y /\ _ |- context[Coqlib.zeq ?X ?Y] =>
