verifier/simulation/correct_bpf_verifier_opcode_alu64_imm.v
@@ -20,40 +20,80 @@ bpf_verifier_opcode_alu64_imm
 *)
 Open Scope Z_scope.
 
-Lemma bpf_verifier_opcode_alu64_imm_match:
-  forall c
-    (Halu : match c with
-       | 7%nat => ADD64_IMM
-       | 23%nat => SUB64_IMM
-       | 39%nat => MUL64_IMM
-       | 55%nat => DIV64_IMM
-       | 71%nat => OR64_IMM
-       | 87%nat => AND64_IMM
-       | 103%nat => LSH64_IMM
-       | 119%nat => RSH64_IMM
-       | 135%nat => NEG64_IMM
-       | 151%nat => MOD64_IMM
-       | 167%nat => XOR64_IMM
-       | 183%nat => MOV64_IMM
-       | 199%nat => ARSH64_IMM
-       | _ => ALU64_IMM_ILLEGAL
-       end = ALU64_IMM_ILLEGAL),
-          7   <> (Z.of_nat c) /\
-          23  <> (Z.of_nat c) /\
-          39  <> (Z.of_nat c) /\
-          55  <> (Z.of_nat c) /\
-          71  <> (Z.of_nat c) /\
-          87  <> (Z.of_nat c) /\
-          103 <> (Z.of_nat c) /\
-          119 <> (Z.of_nat c) /\
-          135 <> (Z.of_nat c) /\
-          151 <> (Z.of_nat c) /\
-          167 <> (Z.of_nat c) /\
-          183 <> (Z.of_nat c) /\
-          199 <> (Z.of_nat c).
+Definition opcode_alu64_imm_if (op: nat) : opcode_alu64_imm :=
+  if Nat.eqb op 7%nat then ADD64_IMM
+  else if Nat.eqb op 23%nat then SUB64_IMM
+  else if Nat.eqb op 39%nat then MUL64_IMM
+  else if Nat.eqb op 55%nat then DIV64_IMM
+  else if Nat.eqb op 71%nat then OR64_IMM
+  else if Nat.eqb op 87%nat then AND64_IMM
+  else if Nat.eqb op 103%nat then LSH64_IMM
+  else if Nat.eqb op 119%nat then RSH64_IMM
+  else if Nat.eqb op 135%nat then NEG64_IMM
+  else if Nat.eqb op 151%nat then MOD64_IMM
+  else if Nat.eqb op 167%nat then XOR64_IMM
+  else if Nat.eqb op 183%nat then MOV64_IMM
+  else if Nat.eqb op 199%nat then ARSH64_IMM
+  else ALU64_IMM_ILLEGAL.
+
+Lemma opcode_alu64_imm_eqb_eq : forall a b,
+    opcode_alu64_imm_eqb a b = true -> a = b.
+Proof.
+  destruct a,b ; simpl ;congruence.
+Qed.
+
+Lemma lift_opcode_alu64_imm :
+  forall (E: nat -> opcode_alu64_imm)
+         (F: nat -> opcode_alu64_imm) n,
+    ((fun n => opcode_alu64_imm_eqb (E n) (F n) = true) n) <->
+      (((fun n => opcode_alu64_imm_eqb (E n) (F n)) n) = true).
 Proof.
   intros.
-  do 200 (destruct c; [inversion Halu; split_conj | ]).
+  simpl. reflexivity.
+Qed.
+
+Lemma byte_to_opcode_alu64_imm_if_same:
+  forall (op: nat),
+    (op <= 255)%nat ->
+    nat_to_opcode_alu64_imm op = opcode_alu64_imm_if op.
+Proof.
+  intros.
+  unfold nat_to_opcode_alu64_imm, opcode_alu64_imm_if.
+  apply opcode_alu64_imm_eqb_eq.
+  match goal with
+  | |- ?A = true => set (P := A)
+  end.
+  pattern op in P.
+  match goal with
+  | P := ?F op |- _=>
+      apply (Forall_exec_spec F 255)
+  end.
+  vm_compute.
+  reflexivity.
+  assumption.
+Qed.
+
+Lemma bpf_verifier_opcode_alu64_imm_match:
+  forall op
+    (Hop: (op <= 255)%nat)
+    (Halu : nat_to_opcode_alu64_imm op = ALU64_IMM_ILLEGAL),
+          7   <> (Z.of_nat op) /\
+          23  <> (Z.of_nat op) /\
+          39  <> (Z.of_nat op) /\
+          55  <> (Z.of_nat op) /\
+          71  <> (Z.of_nat op) /\
+          87  <> (Z.of_nat op) /\
+          103 <> (Z.of_nat op) /\
+          119 <> (Z.of_nat op) /\
+          135 <> (Z.of_nat op) /\
+          151 <> (Z.of_nat op) /\
+          167 <> (Z.of_nat op) /\
+          183 <> (Z.of_nat op) /\
+          199 <> (Z.of_nat op).
+Proof.
+  intros.
+  rewrite byte_to_opcode_alu64_imm_if_same in Halu; auto.
+  unfold opcode_alu64_imm_if in Halu.
   change 7   with (Z.of_nat 7%nat).
   change 23  with (Z.of_nat 23%nat).
   change 39  with (Z.of_nat 39%nat).
@@ -67,11 +107,25 @@ Proof.
   change 167 with (Z.of_nat 167%nat).
   change 183 with (Z.of_nat 183%nat).
   change 199 with (Z.of_nat 199%nat).
-  repeat (split; [intro Hfalse; apply Nat2Z.inj in Hfalse; inversion Hfalse |]).
-  intro Hfalse; apply Nat2Z.inj in Hfalse; inversion Hfalse.
+
+  repeat match goal with
+  | H : (if ?X then _ else _) = _ |- _ /\ _ =>
+    split; [destruct X eqn: Hnew; [inversion H |
+      rewrite Nat.eqb_neq in Hnew;
+      intro Hfalse; apply Hnew;
+      symmetry in Hfalse;
+      apply Nat2Z.inj in Hfalse;
+      assumption]
+    | destruct X eqn: Hnew; [inversion H| clear Hnew]]
+  | H : (if ?X then _ else _) = _ |- _ =>
+    destruct X eqn: Hnew; [inversion H |
+      rewrite Nat.eqb_neq in Hnew;
+      intro Hfalse; apply Hnew;
+      symmetry in Hfalse;
+      apply Nat2Z.inj in Hfalse;
+      assumption]
+  end.
 Qed.
-
-
 
 Section Bpf_verifier_opcode_alu64_imm.
   Context {S:special_blocks}.
@@ -810,8 +864,7 @@ Ltac correct_forward L :=
 
         unfold select_switch.
         unfold select_switch_case.
-        unfold nat_to_opcode_alu64_imm in Halu.
-        apply bpf_verifier_opcode_alu64_imm_match in Halu.
+        apply bpf_verifier_opcode_alu64_imm_match in Halu; auto.
         destruct Halu as (Hfirst & Halu). eapply Coqlib.zeq_false in Hfirst. rewrite Hfirst; clear Hfirst.
         repeat match goal with
         | H: ?X <> ?Y /\ _ |- context[Coqlib.zeq ?X ?Y] =>
