verifier/simulation/correct_bpf_verifier_opcode_alu64_reg.v
@@ -20,38 +20,78 @@ bpf_verifier_opcode_alu64_reg
 *)
 Open Scope Z_scope.
 
-Lemma bpf_verifier_opcode_alu64_reg_match:
-  forall c
-  (Halu : match c with
-       | 15%nat => ADD64_REG
-       | 31%nat => SUB64_REG
-       | 47%nat => MUL64_REG
-       | 63%nat => DIV64_REG
-       | 79%nat => OR64_REG
-       | 95%nat => AND64_REG
-       | 111%nat => LSH64_REG
-       | 127%nat => RSH64_REG
-       | 159%nat => MOD64_REG
-       | 175%nat => XOR64_REG
-       | 191%nat => MOV64_REG
-       | 207%nat => ARSH64_REG
-       | _ => ALU64_REG_ILLEGAL
-       end = ALU64_REG_ILLEGAL),
-      15  <> (Z.of_nat c) /\
-      31  <> (Z.of_nat c) /\
-      47  <> (Z.of_nat c) /\
-      63  <> (Z.of_nat c) /\
-      79  <> (Z.of_nat c) /\
-      95  <> (Z.of_nat c) /\
-      111 <> (Z.of_nat c) /\
-      127 <> (Z.of_nat c) /\
-      159 <> (Z.of_nat c) /\
-      175 <> (Z.of_nat c) /\
-      191 <> (Z.of_nat c) /\
-      207 <> (Z.of_nat c).
+Definition opcode_alu64_reg_if (op: nat) : opcode_alu64_reg :=
+  if Nat.eqb op 15%nat then ADD64_REG
+  else if Nat.eqb op 31%nat then SUB64_REG
+  else if Nat.eqb op 47%nat then MUL64_REG
+  else if Nat.eqb op 63%nat then DIV64_REG
+  else if Nat.eqb op 79%nat then OR64_REG
+  else if Nat.eqb op 95%nat then AND64_REG
+  else if Nat.eqb op 111%nat then LSH64_REG
+  else if Nat.eqb op 127%nat then RSH64_REG
+  else if Nat.eqb op 159%nat then MOD64_REG
+  else if Nat.eqb op 175%nat then XOR64_REG
+  else if Nat.eqb op 191%nat then MOV64_REG
+  else if Nat.eqb op 207%nat then ARSH64_REG
+  else ALU64_REG_ILLEGAL.
+
+Lemma opcode_alu64_reg_eqb_eq : forall a b,
+    opcode_alu64_reg_eqb a b = true -> a = b.
+Proof.
+  destruct a,b ; simpl ;congruence.
+Qed.
+
+Lemma lift_opcode_alu64_reg :
+  forall (E: nat -> opcode_alu64_reg)
+         (F: nat -> opcode_alu64_reg) n,
+    ((fun n => opcode_alu64_reg_eqb (E n) (F n) = true) n) <->
+      (((fun n => opcode_alu64_reg_eqb (E n) (F n)) n) = true).
 Proof.
   intros.
-  do 208 (destruct c; [inversion Halu; split_conj | ]).
+  simpl. reflexivity.
+Qed.
+
+Lemma byte_to_opcode_alu64_reg_if_same:
+  forall (op: nat),
+    (op <= 255)%nat ->
+    nat_to_opcode_alu64_reg op = opcode_alu64_reg_if op.
+Proof.
+  intros.
+  unfold nat_to_opcode_alu64_reg, opcode_alu64_reg_if.
+  apply opcode_alu64_reg_eqb_eq.
+  match goal with
+  | |- ?A = true => set (P := A)
+  end.
+  pattern op in P.
+  match goal with
+  | P := ?F op |- _=>
+      apply (Forall_exec_spec F 255)
+  end.
+  vm_compute.
+  reflexivity.
+  assumption.
+Qed.
+
+Lemma bpf_verifier_opcode_alu64_reg_match:
+  forall op
+    (Hop: (op <= 255)%nat)
+    (Halu : nat_to_opcode_alu64_reg op = ALU64_REG_ILLEGAL),
+      15  <> (Z.of_nat op) /\
+      31  <> (Z.of_nat op) /\
+      47  <> (Z.of_nat op) /\
+      63  <> (Z.of_nat op) /\
+      79  <> (Z.of_nat op) /\
+      95  <> (Z.of_nat op) /\
+      111 <> (Z.of_nat op) /\
+      127 <> (Z.of_nat op) /\
+      159 <> (Z.of_nat op) /\
+      175 <> (Z.of_nat op) /\
+      191 <> (Z.of_nat op) /\
+      207 <> (Z.of_nat op).
+Proof.
+  intros.
+  rewrite byte_to_opcode_alu64_reg_if_same in Halu; auto.
+  unfold opcode_alu64_reg_if in Halu.
   change 15  with (Z.of_nat 15%nat).
   change 31  with (Z.of_nat 31%nat).
   change 47  with (Z.of_nat 47%nat).
@@ -64,8 +104,24 @@ Proof.
   change 175 with (Z.of_nat 175%nat).
   change 191 with (Z.of_nat 191%nat).
   change 207 with (Z.of_nat 207%nat).
-  repeat (split; [intro Hfalse; apply Nat2Z.inj in Hfalse; inversion Hfalse |]).
-  intro Hfalse; apply Nat2Z.inj in Hfalse; inversion Hfalse.
+
+  repeat match goal with
+  | H : (if ?X then _ else _) = _ |- _ /\ _ =>
+    split; [destruct X eqn: Hnew; [inversion H |
+      rewrite Nat.eqb_neq in Hnew;
+      intro Hfalse; apply Hnew;
+      symmetry in Hfalse;
+      apply Nat2Z.inj in Hfalse;
+      assumption]
+    | destruct X eqn: Hnew; [inversion H| clear Hnew]]
+  | H : (if ?X then _ else _) = _ |- _ =>
+    destruct X eqn: Hnew; [inversion H |
+      rewrite Nat.eqb_neq in Hnew;
+      intro Hfalse; apply Hnew;
+      symmetry in Hfalse;
+      apply Nat2Z.inj in Hfalse;
+      assumption]
+  end.
 Qed.
 
 Section Bpf_verifier_opcode_alu64_reg.
@@ -1002,8 +1058,7 @@ Ltac correct_forward L :=
 
         unfold select_switch.
         unfold select_switch_case.
-        unfold nat_to_opcode_alu64_reg in Halu.
-        apply bpf_verifier_opcode_alu64_reg_match in Halu.
+        apply bpf_verifier_opcode_alu64_reg_match in Halu; auto.
         destruct Halu as (Hfirst & Halu). eapply Coqlib.zeq_false in Hfirst. rewrite Hfirst; clear Hfirst.
         repeat match goal with
         | H: ?X <> ?Y /\ _ |- context[Coqlib.zeq ?X ?Y] =>
